src/basic/FStar.Options.fsti
@@ -186,6 +186,7 @@ val quake_keep                  : unit    -> bool
 val query_cache                 : unit    -> bool
 val query_stats                 : unit    -> bool
 val read_checked_file           : unit    -> option string
+val read_krml_file              : unit    -> option string
 val record_hints                : unit    -> bool
 val record_options              : unit    -> bool
 val retry                       : unit    -> bool
